WIP get closedness assumptions right

theories/unary_lr.v
@@ -33,10 +33,10 @@ Section logrel.
 
   Program Definition def_interp_vmem (interp : listVlC -n> D) :
     listVlC -n> dmC -n> iProp Σ :=
-    λne ρ d, (∃ vmem, ⌜d = dvl vmem⌝ ∧ ▷ interp ρ vmem)%I.
+    λne ρ d, (⌜ fv_n d 0 ⌝ ∗ ∃ vmem, ⌜d = dvl vmem⌝ ∧ ▷ interp ρ vmem)%I.
 
   Program Definition interp_vmem l (interp : listVlC -n> D) : listVlC -n> D :=
-    λne ρ v, (∃ d, ⌜v @ l ↘ d⌝ ∧ def_interp_vmem interp ρ d)%I.
+    λne ρ v, (⌜ fv_n_vl v 0 ⌝ ∗ ∃ d, ⌜v @ l ↘ d⌝ ∧ def_interp_vmem interp ρ d)%I.
 
   Definition idm_proj_semtype d σ' (φ : listVlC -n> D) : iProp Σ :=
     (∃ γ, ⌜ d = dtysem σ' γ ⌝ ∗ γ ⤇ (λ vs w, φ vs w))%I.
@@ -46,14 +46,14 @@ Section logrel.
   Program Definition def_interp_tmem (interp1 interp2 : listVlC -n> D) :
     listVlC -n> dmC -n> iProp Σ :=
     λne ρ d,
-    (∃ φ σ, (d ↗ σ , φ) ∗
+    (⌜ fv_n d 0 ⌝ ∗ ∃ φ σ, (d ↗ σ , φ) ∗
        □ ((∀ v, ▷ interp1 ρ v → ▷ □ φ σ v) ∗
           (∀ v, ▷ φ σ v → ▷ interp2 ρ v) ∗
           (∀ v, interp1 ρ v → interp2 ρ v)))%I.
 
   Program Definition interp_tmem l (interp1 interp2 : listVlC -n> D) : listVlC -n> D :=
     λne ρ v,
-    (∃ d, ⌜ v @ l ↘ d ⌝ ∧ def_interp_tmem interp1 interp2 ρ d)%I.
+    (⌜ fv_n_vl v 0 ⌝ ∗ ∃ d, ⌜ v @ l ↘ d ⌝ ∧ def_interp_tmem interp1 interp2 ρ d)%I.
 
   Program Definition interp_expr (φ : listVlC -n> D) : listVlC -n> tmC -n> iProp Σ :=
     λne ρ t, WP t {{ φ ρ }} %I.
@@ -65,11 +65,11 @@ Section logrel.
     λne ρ v, (interp1 ρ v ∨ interp2 ρ v) %I.
 
   Program Definition interp_later (interp : listVlC -n> D) : listVlC -n> D :=
-    λne ρ v, (▷ (interp ρ v)) % I.
+    λne ρ v, (⌜ fv_n_vl v 0 ⌝ ∗ ▷ (interp ρ v)) % I.
 
   Program Definition interp_nat : listVlC -n> D := λne ρ v, (∃ n, ⌜v = vnat n⌝) %I.
 
-  Program Definition interp_top : listVlC -n> D := λne ρ v, True%I.
+  Program Definition interp_top : listVlC -n> D := λne ρ v, ⌜ fv_n_vl v 0 ⌝%I.
 
   Program Definition interp_bot : listVlC -n> D := λne ρ v, False%I.
 
@@ -87,7 +87,7 @@ Section logrel.
    *)
   Program Definition interp_forall (interp1 interp2 : listVlC -n> D) : listVlC -n> D :=
     λne ρ v,
-    (□ ∀ w, interp1 ρ w -∗ interp_expr interp2 (w :: ρ) (tapp (tv v) (tv w)))%I.
+    (⌜ fv_n_vl v 0 ⌝ ∗ □ ∀ w, interp1 ρ w -∗ interp_expr interp2 (w :: ρ) (tapp (tv v) (tv w)))%I.
 
   Program Definition interp_mu (interp : listVlC -n> D) : listVlC -n> D :=
     λne ρ v, interp (v::ρ) v.
@@ -158,6 +158,24 @@ Section logrel.
     Persistent (def_interp T l ρ d).
   Proof. revert ρ d; induction T; simpl; try apply _. Qed.
 
+  Require Import Dot.synLemmas.
+
+  Lemma interp_v_closed T v ρ: (interp T ρ v → ⌜ fv_n_vl v 0 ⌝)%I.
+  Proof.
+    iInduction T as [] "IHT" forall (ρ v); iIntros "#HT //="; try by iDestruct "HT" as "[% _]".
+    (* move: ρ v; induction T; iIntros (ρ v) "HT //="; try solve [by iDestruct "HT" as "[% _]"]. *)
+    - iDestruct "HT" as "[#HT1 #HT2]". by iApply "IHT".
+    - iDestruct "HT" as "[#HT1 | #HT2]"; by [iApply "IHT" | iApply "IHT1"].
+    - by iApply "IHT".
+    - iDestruct "HT" as "[#HT2 _]". by iApply "IHT1".
+    - iDestruct "HT" as (n) "%"; subst. iPureIntro. solve_fv_congruence.
+  Qed.
+
+  Lemma def_interp_v_closed T d l ρ: (def_interp T l ρ d → ⌜ fv_n d 0 ⌝)%I.
+  Proof.
+    iInduction T as [] "IH" forall (ρ d); iIntros "#HT //="; by iDestruct "HT" as "[% [% _]]".
+  Qed.
+
   Program Definition defs_interp_and
              (interp1 : listVlC -n> dmsC -n> iProp Σ)
              (interp2: label -> listVlC -n> dmC -n> iProp Σ)
@@ -171,7 +189,7 @@ Section logrel.
   Program Fixpoint defs_interp (T: ty) : listVlC -n> dmsC -n> iProp Σ :=
     match T with
     | TAnd T1 T2 => defs_interp_and (defs_interp T1) (def_interp T2)
-    | TTop => λne ρ ds, True
+    | TTop => λne ρ ds, ⌜ fv_n ds 0 ⌝
     | _ => λne ρ ds, False
     end % I.
 
@@ -179,6 +197,16 @@ Section logrel.
     Persistent (defs_interp T ρ ds).
   Proof.
     revert ds ρ; induction T; simpl; intros; try case_match; try apply _.
+  Qed.
+
+  Lemma defs_interp_v_closed T ds ρ: (defs_interp T ρ ds → ⌜ fv_n ds 0 ⌝)%I.
+  Proof.
+    iInduction T as [] "IH" forall (ρ ds); iIntros "#HT //=".
+    destruct ds. done.
+    iDestruct "HT" as "[HT1 HT2]".
+    iPoseProof ("IH" with "HT1") as "%".
+    iPoseProof (def_interp_v_closed with "HT2") as "%".
+    iPureIntro. by apply fv_dms_cons.
   Qed.
 
   Fixpoint interp_env (Γ : ctx) (vs : vls) : iProp Σ :=
@@ -201,43 +229,74 @@ Section logrel.
     - simpl. destruct ρ; rewrite /Persistent; eauto.
   Qed.
 
-  (* Definitions for semantic (definition) (sub)typing *)
+  (** Definitions for semantic (definition) (sub)typing *)
+  (** Since [⟦Γ⟧* ρ] might be impossible, we must require closedness explicitly. *)
   Definition idtp Γ T l d : iProp Σ :=
-    (□∀ ρ, ⟦Γ⟧* ρ → def_interp T l ρ d.|[to_subst ρ])%I.
+    (⌜ fv_n d (length Γ) ⌝ ∗ □∀ ρ, ⟦Γ⟧* ρ → def_interp T l ρ d.|[to_subst ρ])%I.
   Global Arguments idtp /.
+  Notation "Γ ⊨d { l = d } : T" := (idtp Γ T l d) (at level 64, l, d, T at next level).
+
+  Lemma idtp_closed Γ T l d: (Γ ⊨d {l = d} : T → ⌜ fv_n d (length Γ) ⌝)%I.
+  Proof. iIntros "[$ _]". Qed.
 
   Definition idstp Γ T ds : iProp Σ :=
-    (□∀ ρ, ⟦Γ⟧* ρ → defs_interp T ρ ds.|[to_subst ρ])%I.
+    (⌜ fv_n ds (length Γ) ⌝ ∗ □∀ ρ, ⟦Γ⟧* ρ → defs_interp T ρ ds.|[to_subst ρ])%I.
   Global Arguments idstp /.
+  Notation "Γ ⊨ds ds : T" := (idstp Γ T ds) (at level 74, ds, T at next level).
+
+  Lemma idstp_closed Γ T ds: (Γ ⊨ds ds : T → ⌜ fv_n ds (length Γ) ⌝)%I.
+  Proof. iIntros "[$ _]". Qed.
 
   Notation "⟦ T ⟧ₑ" := (interp_expr (interp T)).
 
   (* Really needed? Try to stop using it. *)
-  Definition ivtp Γ T v : iProp Σ := (□∀ ρ, ⟦Γ⟧* ρ → ⟦T⟧ ρ v.[to_subst ρ])%I.
+  Definition ivtp Γ T v : iProp Σ := (⌜ fv_n_vl v (length Γ) ⌝ ∗ □∀ ρ, ⟦Γ⟧* ρ → ⟦T⟧ ρ v.[to_subst ρ])%I.
   Global Arguments ivtp /.
 
-  Definition ietp Γ T e : iProp Σ := (□∀ ρ, ⟦Γ⟧* ρ → ⟦T⟧ₑ ρ (e.|[to_subst ρ]))%I.
+  Definition ietp Γ T e : iProp Σ := (⌜ fv_n e (length Γ) ⌝ ∗ □∀ ρ, ⟦Γ⟧* ρ → ⟦T⟧ₑ ρ (e.|[to_subst ρ]))%I.
   Global Arguments ietp /.
+  Notation "Γ ⊨ e : T" := (ietp Γ T e) (at level 74, e, T at next level).
+
+  Lemma ietp_closed Γ T e: (Γ ⊨ e : T → ⌜ fv_n e (length Γ) ⌝)%I.
+  Proof. iIntros "[$ _]". Qed.
 
   Definition step_indexed_ietp Γ T e i: iProp Σ :=
-    (□∀ ρ, ⟦Γ⟧* ρ → ▷^i ⟦T⟧ₑ ρ (e.|[to_subst ρ]))%I.
+    (⌜ fv_n e (length Γ) ⌝ ∗ □∀ ρ, ⟦Γ⟧* ρ → ▷^i ⟦T⟧ₑ ρ (e.|[to_subst ρ]))%I.
   Global Arguments step_indexed_ietp /.
+  Notation "Γ ⊨ e : T , i" := (step_indexed_ietp Γ T e i) (at level 74, e, T at next level).
 
-  (* Subtyping. Defined on (values). *)
+  Lemma step_indexed_ietp_closed Γ T e i: (Γ ⊨ e : T, i → ⌜ fv_n e (length Γ) ⌝)%I.
+  Proof. iIntros "[$ _]". Qed.
+
+  (** Subtyping. Defined on values. *)
   Definition ivstp Γ T1 T2: iProp Σ := (□∀ ρ v, ⟦Γ⟧* ρ → ⟦T1⟧ ρ v → ⟦T2⟧ ρ v)%I.
   Global Arguments ivstp /.
 
+  (** Indexed Subtyping. Defined on closed values. We must require closedness
+      explicitly, since closedness now does not follow from being well-typed later. *)
   Definition step_indexed_ivstp Γ T1 T2 i j: iProp Σ :=
-    (□∀ ρ v, ⟦Γ⟧*ρ -∗ (▷^i ⟦T1⟧ ρ v) → ▷^j ⟦T2⟧ ρ v)%I.
+    (□∀ ρ v, ⌜ fv_n_vl v 0 ⌝ → ⟦Γ⟧*ρ → (▷^i ⟦T1⟧ ρ v) → ▷^j ⟦T2⟧ ρ v)%I.
   Global Arguments step_indexed_ivstp /.
+
+  Global Instance idtp_persistent Γ T l d: Persistent (idtp Γ T l d) := _.
+  Global Instance idstp_persistent Γ T ds: Persistent (idstp Γ T ds) := _.
+  Global Instance ietp_persistent Γ T e : Persistent (ietp Γ T e) := _.
+  Global Instance step_indexed_ietp_persistent Γ T e i : Persistent (step_indexed_ietp Γ T e i) := _.
+  Global Instance step_indexed_ivstp_persistent Γ T1 T2 i j : Persistent (step_indexed_ivstp Γ T1 T2 i j) := _.
+  Global Instance ivstp_persistent Γ T1 T2 : Persistent (ivstp Γ T1 T2) := _.
 End logrel.
 
 Notation "⟦ T ⟧" := (interp T).
 Notation "⟦ Γ ⟧*" := (interp_env Γ).
 Notation "⟦ T ⟧ₑ" := (interp_expr (interp T)).
 
+(** Single-definition typing *)
+Notation "Γ ⊨d d : T" := (idtp Γ T d) (at level 74, d, T at next level).
+(** Multi-definition typing *)
 Notation "Γ ⊨ds ds : T" := (idstp Γ T ds) (at level 74, ds, T at next level).
+(** Expression typing *)
 Notation "Γ ⊨ e : T" := (ietp Γ T e) (at level 74, e, T at next level).
+(** Indexed expression typing *)
 Notation "Γ ⊨ e : T , i" := (step_indexed_ietp Γ T e i) (at level 74, e, T at next level).
 
 Notation "Γ ⊨ T1 <: T2" := (ivstp Γ T1 T2) (at level 74, T1, T2 at next level).
@@ -249,16 +308,18 @@ Section logrel_lemmas.
   Context `{HdotG: dotG Σ}.
 
   Lemma iterate_TLater_later i T ρ v:
-    (⟦ iterate TLater i T ⟧ ρ v = ▷^i ⟦ T ⟧ ρ v)%I.
+    fv_n_vl v 0 →
+    ⟦ iterate TLater i T ⟧ ρ v ≡ (▷^i ⟦ T ⟧ ρ v)%I.
   Proof.
-    elim: i => [|i IHi] //. by rewrite iterate_S /= IHi.
+    elim: i => [|i IHi] // => Hcl. rewrite iterate_S /= IHi //.
+    iSplit; by [iIntros "#[_ $]" | iIntros "$"].
   Qed.
 
-  Lemma interp_weaken Δ1 Π Δ2 τ :
-    ⟦ τ.|[upn (length Δ1) (ren (+ length Π))] ⟧ (Δ1 ++ Π ++ Δ2)
-    ≡ ⟦ τ ⟧ (Δ1 ++ Δ2).
+  Lemma interp_weaken ρ1 ρ2 ρ3 τ :
+    ⟦ τ.|[upn (length ρ1) (ren (+ length ρ2))] ⟧ (ρ1 ++ ρ2 ++ ρ3)
+    ≡ ⟦ τ ⟧ (ρ1 ++ ρ3).
   Proof.
-    revert Δ1 Π Δ2; induction τ=> Δ1 Π Δ2 w; simpl; trivial; asimpl;
+    revert ρ1 ρ2 ρ3; induction τ=> ρ1 ρ2 ρ3 w; simpl; trivial; asimpl;
                                     rewrite ?to_subst_weaken.
     all: try solve [properness; trivial;
                     apply IHτ || apply IHτ1 || apply IHτ2 ||
@@ -269,18 +330,18 @@ Section logrel_lemmas.
      ⟦ τ.|[ren (+1)] ⟧ (v :: ρ) ≡ ⟦ τ ⟧ ρ.
   Proof. apply (interp_weaken [] [v]). Qed.
 
-  Lemma interp_subst_up Δ1 Δ2 τ v:
-    ⟦ τ.|[upn (length Δ1) (v.[ren (+length Δ2)] .: ids)] ⟧ (Δ1 ++ Δ2)
-    ≡ ⟦ τ ⟧ (Δ1 ++ v :: Δ2).
+  Lemma interp_subst_up ρ1 ρ2 τ v:
+    ⟦ τ.|[upn (length ρ1) (v.[ren (+length ρ2)] .: ids)] ⟧ (ρ1 ++ ρ2)
+    ≡ ⟦ τ ⟧ (ρ1 ++ v :: ρ2).
   Proof.
-    revert Δ1 Δ2; induction τ=> Δ1 Δ2 w; simpl; trivial; asimpl;
+    revert ρ1 ρ2; induction τ=> ρ1 ρ2 w; simpl; trivial; asimpl;
                                     rewrite ?to_subst_up.
     all: try solve [properness; trivial;
                     apply IHτ || apply IHτ1 || apply IHτ2 ||
                           apply (IHτ2 (_ :: _)) || apply (IHτ (_ :: _))].
   Qed.
 
-  Lemma interp_subst Δ2 τ v1 v2 : ⟦ τ.|[v1.[ren (+length Δ2)]/] ⟧ Δ2 v2 ≡ ⟦ τ ⟧ (v1 :: Δ2) v2.
+  Lemma interp_subst ρ τ v1 v2 : ⟦ τ.|[v1.[ren (+length ρ)]/] ⟧ ρ v2 ≡ ⟦ τ ⟧ (v1 :: ρ) v2.
   Proof. apply (interp_subst_up []). Qed.
 
   Context Γ.
@@ -288,36 +349,32 @@ Section logrel_lemmas.
   Lemma semantic_typing_uniform_step_index T e i:
     (Γ ⊨ e : T → Γ ⊨ e : T,i)%I.
   Proof.
-    induction i; iIntros "#H"; iModIntro; iIntros (ρ) "#HΓ".
-    - by iApply "H".
-    - iModIntro. by iApply IHi.
+    iIntros "[$ #H] !>" (ρ) "#HΓ".
+    iInduction i as [|i] "IHi". by iApply "H". iApply "IHi".
   Qed.
 
   Lemma interp_env_lookup ρ T x:
     Γ !! x = Some T →
     (⟦ Γ ⟧* ρ → ⟦ T.|[ren (+x)] ⟧ ρ (to_subst ρ x))%I.
   Proof.
-    intros Hx.
-    iIntros "* #Hg".
+    iIntros (Hx) "* #Hg".
     iInduction Γ as [|T' Γ'] "IHL" forall (x ρ Hx); simpl; try solve [inversion Hx].
     destruct ρ; try by iExFalso.
     iDestruct "Hg" as "[̋Hg Ht]".
-    case : x Hx.
-    - move => [ -> ] /=. iSpecialize ("IHL" $! 0). by asimpl.
-    - move => /= x Hx.
-      rewrite to_subst_cons /=.
+    case: x Hx => /= [|x] Hx.
+    - move: Hx => [ -> ]. iSpecialize ("IHL" $! 0). by asimpl.
+    - rewrite to_subst_cons /=.
       iAssert (⟦ T.|[ren (+x)] ⟧ ρ (to_subst ρ x)) as "#Hv". by iApply "IHL".
-      iPoseProof (interp_weaken [] [v] ρ with "Hv") as "H". by asimpl.
+      iPoseProof (interp_weaken [] [v] ρ with "Hv") as "H"; asimpl. iExact "H".
   Qed.
 
   Lemma interp_env_len_agree ρ:
     (⟦ Γ ⟧* ρ → ⌜ length ρ = length Γ ⌝)%I.
   Proof.
-    iIntros "#HG".
-    iInduction Γ as [|τ Γ'] "IHΓ" forall (ρ); destruct ρ; simpl; trivial.
-    - iDestruct "HG" as "%". discriminate.
-    - iDestruct "HG" as "[HG' Hv]".
-      by iDestruct ("IHΓ" $! ρ with "HG'") as "->".
+    iInduction Γ as [|τ Γ'] "IHΓ" forall (ρ); destruct ρ => //=.
+    iIntros "#[HG Hv]".
+    Fail iRewrite ("IHΓ" $! ρ with "HG").
+    by iDestruct ("IHΓ" $! ρ with "HG") as "->".
   Qed.
 
   Lemma interp_subst_all ρ τ v:
@@ -326,47 +383,92 @@ Section logrel_lemmas.
     elim: ρ τ => /= [|w ρ IHρ] τ Hwρcl; asimpl; first by [].
     assert (fv_n_vl w 0 /\ Forall (λ v, fv_n_vl v 0) ρ) as [Hwcl Hρcl]. by inversion Hwρcl.
     specialize (IHρ (τ.|[w/]) Hρcl).
-    asimpl in IHρ.
-    by rewrite -interp_subst closed_subst_vl_id -?IHρ ?closed_subst_vl_id.
+    asimpl in IHρ. move: IHρ. rewrite closed_subst_vl_id// => IHρ.
+    rewrite IHρ -interp_subst closed_subst_vl_id //.
   Qed.
 
   Lemma to_subst_interp T ρ v w: cl_ρ ρ → fv_n_vl v (length ρ) →
     ⟦ T.|[v/] ⟧ ρ w ≡ ⟦ T.|[v.[to_subst ρ]/] ⟧ ρ w.
   Proof.
     intros Hclρ Hclv.
-    rewrite -(interp_subst_all ρ (T.|[v/])) -?(interp_subst_all ρ (T.|[v.[to_subst ρ]/])); trivial.
-    asimpl. do 5 f_equiv.
-    apply Hclv.
-    intros x Hl.
-    asimpl.
-    rewrite closed_subst_vl_id; trivial.
-    by apply closed_to_subst.
+    assert (v.[to_subst ρ] = v.[to_subst ρ >> to_subst ρ]) as Hrew. {
+      apply Hclv.
+      intros x Hl.
+      asimpl.
+      rewrite closed_subst_vl_id //. by apply closed_to_subst.
+    }
+    rewrite -(interp_subst_all ρ (T.|[v/])) // -(interp_subst_all ρ (T.|[v.[to_subst ρ]/])) //.
+    asimpl. by rewrite -Hrew.
   Qed.
 
-  Lemma interp_subst_closed T v w ρ:
+  Lemma interp_env_ρ_closed ρ: (⟦ Γ ⟧* ρ → ⌜ cl_ρ ρ ⌝)%I.
+  Proof.
+    revert Γ ρ. elim => [|T Γ IHl] [|v ρ] /=; try (by iIntros "%").
+    iIntros "[#HG #HT]".
+    iPoseProof (interp_v_closed with "HT") as "%".
+    iPoseProof (IHl with "HG") as "%".
+    iPureIntro; by constructor.
+  Qed.
+
+  Lemma interp_env_to_subst_closed ρ x: x < length ρ → (⟦ Γ ⟧* ρ → ⌜ fv_n_vl (to_subst ρ x) 0 ⌝)%I.
+  Proof.
+    iIntros (Hl) "#HG". iPoseProof (interp_env_ρ_closed with "HG") as "%".
+    iPureIntro; by apply closed_to_subst.
+  Qed.
+
+  Lemma ietp_closed_vl T v: (Γ ⊨ tv v : T → ⌜ fv_n_vl v (length Γ) ⌝)%I.
+  Proof.
+    iIntros "H".
+    iPoseProof (ietp_closed with "H") as "%". by iPureIntro; apply fv_tv_inv.
+  Qed.
+
+  (* Lemma interp_env_to_subst_closed ρ x: x < length ρ → (⟦ Γ ⟧* ρ → ⌜ fv_n_vl (to_subst ρ x) 0 ⌝)%I. *)
+  (* Proof. *)
+  (*   (* Hint Resolve defs_interp_v_closed def_interp_v_closed interp_v_closed. *) *)
+  (*   revert Γ ρ x. *)
+  (*   elim => [|T Γ IHl] [|v ρ] [|x] /= Hl; try omega; try (iIntros "%"; discriminate); iIntros "[#HG #HT]". *)
+  (*   - iApply interp_v_closed. rewrite to_subst_cons /=. iApply "HT". *)
+  (*   - asimpl. by iApply IHl; first omega. *)
+  (* Qed. *)
+
+  (* Lemma interp_subst_closed T v w ρ: *)
+  (*   fv_n_vl v (length ρ) → *)
+  (*   (⟦ Γ ⟧* ρ → ⟦ T.|[v/] ⟧ ρ w ∗-∗ ⟦ T ⟧ (v.[to_subst ρ] :: ρ) w)%I. *)
+  (* Proof. *)
+  (*   iIntros (Hcl) "#HG". *)
+  (*   iAssert ⌜ cl_ρ ρ ⌝%I as "%". by iApply interp_env_ρ_closed. move: H => Hclρ. *)
+  (*   assert (⟦ T.|[v.[to_subst ρ]/] ⟧ ρ w ≡ ⟦ T.|[v/] ⟧ ρ w) as Hren. by rewrite (to_subst_interp T ρ v w). *)
+  (*   iPoseProof (interp_subst ρ T (v.[to_subst ρ]) w) as "Heq"; asimpl. *)
+  (*   iAssert (⌜ eq_n_s (to_subst ρ >> ren (+length ρ)) (to_subst ρ) (length ρ) ⌝)%I as "%". *)
+  (*   { *)
+  (*     iIntros (x Hxl). *)
+  (*     iPoseProof (interp_env_to_subst_closed ρ x Hxl with "HG") as "%". move: H => Hclx. *)
+  (*     iPureIntro; apply closed_subst_vl_id, Hclx. *)
+  (*   } *)
+  (*   rewrite (Hcl (to_subst ρ >> ren (+length ρ)) (to_subst ρ)) //. *)
+  (*   rewrite Hren. *)
+  (*   iExact "Heq". *)
+  (* Qed. *)
+
+  (* Try giving a simpler proof: *)
+  Lemma interp_subst_closed_aux T v w ρ:
     fv_n_vl v (length ρ) →
     (⟦ Γ ⟧* ρ → ⟦ T.|[v/] ⟧ ρ w ∗-∗ ⟦ T ⟧ (v.[to_subst ρ] :: ρ) w)%I.
   Proof.
-    intro Hcl.
-    assert ((⟦ T.|[v/] ⟧ ρ w = ⟦ T.|[v.[to_subst ρ]/] ⟧ ρ w)) as Hren. admit.
-    iIntros "#HG".
-    iPoseProof (interp_subst ρ T (v.[to_subst ρ]) w) as "Heq"; asimpl.
-    rewrite (Hcl (to_subst ρ >> ren (+length ρ)) (to_subst ρ)).
-    + by rewrite Hren.
-    + intros. asimpl.
-      (* Here we must deduce that entries in ρ are closed. Which isn't true yet. *)
-      admit.
-  Admitted.
+    iIntros (Hcl) "#Hg".
+    iPoseProof (interp_env_ρ_closed ρ with "Hg") as "%"; move: H => Hclρ.
+    iPoseProof (interp_subst ρ T (v.[to_subst ρ]) w) as "Heq"; iEval (asimpl) in "Heq".
+    rewrite (Hcl (to_subst ρ >> ren (+length ρ)) (to_subst ρ)) // -?(to_subst_interp T ρ v w) //.
+    move => x Hlρ. asimpl. by rewrite closed_subst_vl_id; [|apply closed_to_subst].
+  Qed.
 
-  Lemma tp_closed T e: (Γ ⊨ e : T → ⌜ fv_n e (length Γ) ⌝)%I.
-  Admitted.
-
-  Lemma tp_closed_vl T v: (Γ ⊨ tv v : T → ⌜ fv_n_vl v (length Γ) ⌝)%I.
+  Lemma interp_subst_closed T v w ρ:
+    fv_n_vl v (length Γ) →
+    (⟦ Γ ⟧* ρ → ⟦ T.|[v/] ⟧ ρ w ∗-∗ ⟦ T ⟧ (v.[to_subst ρ] :: ρ) w)%I.
   Proof.
-    iIntros "H". iPoseProof (tp_closed with "H") as "%". iPureIntro.
-    move :H.
-    rewrite /fv_n_vl /fv_n /= => Hcl s1 s2 HsEq.
-    specialize (Hcl s1 s2 HsEq). by injectHyps.
+    iIntros (Hcl) "#Hg".
+    iPoseProof (interp_env_len_agree ρ with "Hg") as "%"; move: H => HlenEq; rewrite <- HlenEq in *.
+    by iApply interp_subst_closed_aux.
   Qed.
 
 End logrel_lemmas.
