theories/lr_lemma.v
@@ -1,12 +1,36 @@
 From iris.base_logic Require Import base_logic.
 From iris.proofmode Require Import tactics.
-From iris.program_logic Require Import weakestpre lifting ectxi_language.
+From iris.program_logic Require Import weakestpre.
+
+(** Paolo to Amin: it seems below we might need something vaguely similar to the following. Not sure they're exactly true as stated. *)
+Section wp_extra.
+Context `{irisG Λ Σ}.
+Implicit Types s : stuckness.
+Implicit Types P : iProp Σ.
+Implicit Types Φ : val Λ → iProp Σ.
+Implicit Types v : val Λ.
+Implicit Types e : expr Λ.
+
+(* (** A variant of wp_wand that requires proof of [Φ v -∗ Ψ v] only if [v] is an evaluation result. *) *)
+(* Lemma wp_wand_steps s E e Φ Ψ: *)
+(*     (WP e @ s; E {{ v, Φ v }} -∗ *)
+(*     (** The nsteps premise is wrong for a multithreaded program logic, feel free to use a more accurate one. *)
+(*         This one might be fine for DOT. *) *)
+(*     (∀ v σ1 κ σ2 i, ⌜ nsteps i ([e], σ1) κ ([of_val v], σ2) ⌝ -∗ Φ v -∗ Ψ v)-∗ *)
+(*     WP e @ s; E {{ v, Ψ v }})%I. *)
+(* Admitted. *)
+
+End wp_extra.
+
+From iris.program_logic Require Import lifting language ectxi_language.
 From Dot Require Import tactics unary_lr rules synLemmas.
-
 Implicit Types (L T U: ty) (v: vl) (e: tm) (d: dm) (ds: dms) (Γ : ctx).
-
 Section Sec.
   Context `{HdotG: dotG Σ} Γ.
+
+  Lemma wp_wand_cl e Φ Ψ:
+    (WP e {{ v, Φ v }} -∗ ⌜ fv_n e 0 ⌝ -∗ (∀ v, Φ v -∗ ⌜ fv_n_vl v 0 ⌝ -∗ Ψ v) -∗ WP e {{ v, Ψ v }})%I.
+  Admitted.
 
   Lemma T_Sub e T1 T2 :
     (Γ ⊨ e : T1 →
@@ -14,9 +38,18 @@ Section Sec.
     (*───────────────────────────────*)
     Γ ⊨ e : T2)%I.
   Proof.
-    iIntros "/= * #HeT1 #Hsub !> * #Hg".
-    iApply wp_wand. by iApply "HeT1".
-    iIntros; by iApply "Hsub".
+    iIntros "/= * #[% #HeT1] #Hsub". move: H => Hcle. iFrame "%". iIntros " !> * #Hg".
+    (* match type of wp_wand with *)
+    (* | ?H => let x := eval simpl in H in idtac x *)
+    (* end. *)
+    (* Check wp_wand. *)
+    (* iApply wp_wand. *)
+    iApply (wp_wand_cl (e.|[to_subst ρ]) _ (⟦ T2 ⟧ ρ)).
+    3: {iIntros; iApply "Hsub" => //. }
+    iApply ("HeT1" $! ρ with "Hg").
+    iPoseProof (interp_env_len_agree with "Hg") as "%". move: H => Hlen.
+    iPoseProof (interp_env_ρ_closed with "Hg") as "%". move: H => Hclρ.
+    iPureIntro. rewrite <- Hlen in Hcle. by apply fv_to_subst.
   Qed.
 
   Lemma T_Var x T:
@@ -24,20 +57,20 @@ Section Sec.
     (*──────────────────────*)
     Γ ⊨ tv (var_vl x) : T.|[ren (+x)].
   Proof.
-    move => Hx /=. iIntros "!> * #Hg".
+    iIntros (Hx) "/=". iSplit; eauto using lookup_fv. iIntros "!> * #Hg".
     iApply wp_value'.
     by iApply interp_env_lookup.
   Qed.
 
   Lemma Sub_Refl T i : Γ ⊨ [T, i] <: [T, i].
-  Proof. by iIntros "/= !> * _ HT". Qed.
+  Proof. by iIntros "/= !> **". Qed.
 
   Lemma Sub_Trans T1 T2 T3 i1 i2 i3 : (Γ ⊨ [T1, i1] <: [T2, i2] →
                                        Γ ⊨ [T2, i2] <: [T3, i3] →
                                        Γ ⊨ [T1, i1] <: [T3, i3])%I.
   Proof.
-    iIntros "#Hsub1 #Hsub2 /= !> * #Hg #HT".
-    iApply "Hsub2"; first done. by iApply "Hsub1".
+    iIntros "#Hsub1 #Hsub2 /= !> * % #Hg #HT".
+    iApply "Hsub2" => //. by iApply "Hsub1".
   Qed.
 
   Lemma Sub_Mono e T i :
@@ -46,11 +79,11 @@ Section Sec.
 
   Lemma Later_Sub e T i :
     (Γ ⊨ [TLater T, i] <: [T, S i])%I.
-  Proof. by iIntros "/= !> ** !>". Qed.
+  Proof. by iIntros "/= !>" (ρ v Hclv) "#HG #[Hcl HT] !>". Qed.
 
   Lemma Sub_Later e T i :
     (Γ ⊨ [T, S i] <: [TLater T, i])%I.
-  Proof. by iIntros "/= !> ** !>". Qed.
+  Proof. iIntros "/= !> ** !>". naive_solver. Qed.
 
   Lemma Sub_Index_Incr e T U i j:
     (Γ ⊨ [T, i] <: [U, j] →
@@ -61,15 +94,15 @@ Section Sec.
     (Γ ⊨ e : T, S i →
      Γ ⊨ tskip e : T, i)%I.
   Proof.
-    iIntros "/= #HT !> * #HG".
+    iIntros "/= [% #HT]". iSplit; auto using fv_tskip. iIntros " !> * #HG".
     iApply wp_pure_step_later; auto.
     iSpecialize ("HT" $! ρ with "HG"). by iModIntro.
   Qed.
 
   Lemma And1_Sub T1 T2 i: Γ ⊨ [TAnd T1 T2, i] <: [T1, i].
-  Proof. by iIntros "/= !> * ? [? ?]". Qed.
+  Proof. by iIntros "/= !> * ? ? [? ?]". Qed.
   Lemma And2_Sub T1 T2 i: Γ ⊨ [TAnd T1 T2, i] <: [T2, i].
-  Proof. by iIntros "/= !> * ? [? ?]". Qed.
+  Proof. by iIntros "/= !> * ? ? [? ?]". Qed.
 
   (* Lemma stp_andi T1 T2 ρ v: *)
   (*   ⟦T1⟧ ρ v -∗ *)
@@ -82,9 +115,9 @@ Section Sec.
     Γ ⊨ [S, i] <: [T2, j] -∗
     Γ ⊨ [S, i] <: [TAnd T1 T2, j].
   Proof.
-    iIntros "/= #H1 #H2 !> * #Hg #HS".
-    iSpecialize ("H1" with "Hg HS").
-    iSpecialize ("H2" with "Hg HS").
+    iIntros "/= #H1 #H2 !> * #Hcl #Hg #HS".
+    iSpecialize ("H1" with "Hcl Hg HS").
+    iSpecialize ("H2" with "Hcl Hg HS").
     iModIntro; by iSplit.
   Qed.
 
@@ -97,11 +130,11 @@ Section Sec.
     Γ ⊨ [T1, i] <: [S, j] -∗
     Γ ⊨ [T2, i] <: [S, j] -∗
     Γ ⊨ [TOr T1 T2, i] <: [S, j].
-  Proof. iIntros "/= #H1 #H2 !> * #Hg #[HT1 | HT2]"; by [iApply "H1" | iApply "H2"]. Qed.
+  Proof. iIntros "/= #H1 #H2 !> * #Hcl #Hg #[HT1 | HT2]"; by [iApply "H1" | iApply "H2"]. Qed.
 
   Lemma Sub_Top T i:
     Γ ⊨ [T, i] <: [TTop, i].
-  Proof. by iIntros "!> **". Qed.
+  Proof. by iIntros "!> ** /=". Qed.
 
   Lemma Bot_Sub T i:
     Γ ⊨ [TBot, i] <: [T, i].
@@ -117,7 +150,7 @@ Section Sec.
     (iterate TLater i T1 :: Γ ⊨ [T1, i] <: [T2, j] →
      Γ ⊨ [TMu T1, i] <: [TMu T2, j])%I.
   Proof.
-    iIntros "/= #Hstp !> * #Hg #HT1".
+    iIntros "/= #Hstp !> * % #Hg #HT1".
     iApply ("Hstp" $! (v :: ρ) _);
       rewrite ?iterate_TLater_later //; by iSplit.
   Qed.
@@ -132,7 +165,7 @@ Section Sec.
     (iterate TLater i T1 :: Γ ⊨ [T1, i] <: [T2.|[ren (+1)], j] →
      Γ ⊨ [TMu T1, i] <: [T2, j])%I.
   Proof.
-    iIntros "/= #Hstp !> * #Hg #HT1".
+    iIntros "/= #Hstp !> * % #Hg #HT1".
     iApply (interp_weaken_one v).
     iApply ("Hstp" $! (v :: ρ)); rewrite ?iterate_TLater_later //; by iSplit.
   Qed.
@@ -146,7 +179,7 @@ Section Sec.
     (iterate TLater i T1.|[ren (+1)] :: Γ ⊨ [T1.|[ren (+1)], i] <: [T2, j] →
     Γ ⊨ [T1, i] <: [TMu T2, j])%I.
   Proof.
-    iIntros "/= #Hstp !> * #Hg #HT1".
+    iIntros "/= #Hstp !> * % #Hg #HT1".
     rewrite -(interp_weaken_one v T1 ρ v).
     iApply ("Hstp" $! (_ :: _) _); rewrite ?iterate_TLater_later //; by iSplit.
   Qed.
@@ -157,8 +190,8 @@ Section Sec.
     (*────────────────────────────────────────────────────────────*)
      Γ ⊨ tapp e1 e2 : T2)%I.
   Proof.
-    iIntros "/= #He1 #Hv2 !> * #HG".
-    smart_wp_bind (AppLCtx (e2.|[to_subst ρ])) v "#Hv" "He1".
+    iIntros "/= #[% He1] #[% Hv2]". iSplit; eauto using fv_tapp. iIntros " !> * #HG".
+    smart_wp_bind (AppLCtx (e2.|[to_subst ρ])) v "#[% Hv]" "He1".
     smart_wp_bind (AppRCtx v) w "#Hw" "Hv2".
     iApply wp_mono; [|iApply "Hv"]; auto.
     iIntros (v0) "#H".
@@ -171,11 +204,11 @@ Section Sec.
     (*────────────────────────────────────────────────────────────*)
      Γ ⊨ tapp e1 (tv v2) : T2.|[v2/])%I.
   Proof.
-    iIntros "/= #He1 #Hv2Arg !> * #HG".
-    iAssert (⌜ fv_n_vl v2 (length Γ) ⌝)%I as "%". by iApply tp_closed_vl. rename H into Hcl.
-    iAssert (⌜ length ρ = length Γ ⌝)%I as "%". by iApply interp_env_len_agree. rename H into Hlen.
-    assert (fv_n_vl v2 (length ρ)). by rewrite Hlen.
-    smart_wp_bind (AppLCtx (tv v2.[to_subst ρ])) v "#HvFun" "He1".
+    iIntros "/= #[% He1] #[% Hv2Arg]". move: H H0 => Hcle1 Hclv2. iSplit; eauto using fv_tapp. iIntros " !> * #HG".
+    (* iAssert (⌜ length ρ = length Γ ⌝)%I as "%". by iApply interp_env_len_agree. move: H => Hlen. *)
+    iAssert (⌜ fv_n_vl v2 (length Γ) ⌝)%I as "%". by iPureIntro; apply fv_tv_inv. move: H => Hcl.
+    (* assert (fv_n_vl v2 (length ρ)). by rewrite Hlen. *)
+    smart_wp_bind (AppLCtx (tv v2.[to_subst ρ])) v "#[% HvFun]" "He1".
     iApply wp_wand.
     - iApply fupd_wp.
       iApply "HvFun".
@@ -188,8 +221,19 @@ Section Sec.
     (*─────────────────────────*)
     Γ ⊨ tv (vabs e) : TAll T1 T2)%I.
   Proof.
-    iIntros "/= #HeT !> * #HG".
+    iIntros "/= #[% HeT]". move: H => Hcle.
+    iSplit; eauto using fv_tv, fv_vabs.
+    iIntros " !> * #HG".
+    iPoseProof (interp_env_ρ_closed with "HG") as "%". move: H => Hclρ.
+    iAssert (⌜ length ρ = length Γ ⌝)%I as "%". by iApply interp_env_len_agree. move: H => Hlen.
     iApply wp_value'.
+    iSplit.
+    { 
+      iPureIntro. rewrite <- Hlen in *.
+      pose proof (fv_to_subst (tv (vabs e)) ρ) as Hfv. asimpl in Hfv.
+      (* apply fv_tv_inv, Hfv => //; apply fv_tv, fv_vabs, Hcle. *)
+      eauto using fv_tv_inv, fv_vabs, fv_tv.
+    }
     iIntros "!>" (v) "#Hv".
     iSpecialize ("HeT" $! (v :: ρ)).
     iApply wp_pure_step_later; trivial.
@@ -204,12 +248,12 @@ Section Sec.
     (*─────────────────────────*)
     Γ ⊨ tproj e l : T)%I.
   Proof.
-    iIntros "#HE /= !>" (ρ) "#HG".
-    smart_wp_bind (ProjCtx l) v "#Hv" "HE".
-    iDestruct "Hv" as (d) "[% Hv]".
+    iIntros "#[% HE] /=". iSplit; auto using fv_tproj. iIntros " !>" (ρ) "#HG".
+    smart_wp_bind (ProjCtx l) v "#[% Hv]" "HE".
+    iDestruct "Hv" as (d) "[% [% Hv]]".
     iDestruct "Hv" as (vmem) "[% Hv]".
     simplOpen ds; subst.
-    inversion H; ev; injectHyps.
+    match goal with H: _ @ _ ↘ _ |- _ => inversion H; ev; injectHyps end.
     iApply wp_pure_step_later; eauto.
     by iApply wp_value'.
   Qed.
@@ -227,78 +271,12 @@ Section Sec.
      Γ ⊨ z: mu(x: Tˣ)
    *)
   Lemma ivstp_rec_eq T v:
-    ((∀ ρ1 ρ2, (∀ x, x < length Γ → ρ1 x = ρ2 x) → v.[ρ1] = v.[ρ2]) ->
-    ivtp Γ (TMu T) v ∗-∗
+    (ivtp Γ (TMu T) v ∗-∗
     ivtp Γ T.|[v/] v)%I.
   Proof.
-    intros Hcl.
-    assert (∀ ρ x, x < length Γ
-             → to_subst ρ x = (to_subst ρ >> ren (+strings.length ρ)) x) as H.
-    {
-      (* Needed below: length Γ = length ρ *)
-      asimpl.
-      admit.
-    }
-    iAssert (□(∀ ρ,
-                 ⟦ T.|[v.[to_subst ρ]/] ⟧ ρ v.[to_subst ρ] ∗-∗ ⟦ T.|[v/] ⟧ ρ v.[to_subst ρ]))%I as "#Hren". admit.
-    iSplit; iIntros "/= #Htp !> * #Hg";
-      iSpecialize ("Htp" $! ρ with "Hg"); iSpecialize ("Hren" $! ρ);
-      iPoseProof (interp_subst ρ T (v.[to_subst ρ]) (v.[to_subst ρ])) as "#Hren1"; asimpl; rewrite - (Hcl (to_subst ρ) ); try naive_solver.
-    - iApply "Hren".
-      iApply "Hren1".
-      iApply "Htp".
-    -
-      iApply "Hren1".
-      iApply "Hren".
-      iApply "Htp".
-  Admitted.
-
-  (* Paolo: This is probably false if we don't assume that v is closed; that
-     must either follow from the logical relation or be a separate hypothesis. *)
-  Lemma ivstp_rec_eq_alt T v:
-    ivtp Γ (TMu T) v ≡
-    ivtp Γ T.|[v/] v.
-  Proof.
-    iSplit; iIntros "/= #Htp !> * #Hg";
-      iSpecialize ("Htp" $! ρ).
-    - iSpecialize ("Htp" with "Hg").
-      rewrite -(interp_subst). asimpl.
-      admit.
-    (*   iRewrite "Hren". *)
-    (*   by iApply "Htp". *)
-    (* - iRewrite "Hren" in "Htp". *)
-    (*   by iApply "Htp". *)
-  Admitted.
-
-  (*   (* iIntros "#Hclosed". *) *)
-  (*   iAssert (□ ∀ ρ, interp_env Γ ρ -∗ interp T.|[v/] ρ v.[to_subst ρ] ∗-∗ interp T (v.[to_subst ρ] :: ρ) v.[to_subst ρ])%I as "#Hren". *)
-  (*   (* iAssert (□ ∀ ρ, interp_env Γ ρ -∗ interp T.|[v/] ρ v.[to_subst ρ] ≡ interp T (v :: ρ) v)%I as "#Hren". *) *)
-  (*   { *)
-  (*     iIntros "!> /= * #Hg". *)
-  (*     iPoseProof (interp_subst ρ T (v.[to_subst ρ]) (v.[to_subst ρ])) as "#H". *)
-  (*     iSplit; iIntros "#H2". *)
-  (*     iApply "H". *)
-  (*     asimpl. *)
-  (*     rewrite - (Hcl (to_subst ρ) ). *)
-  (*     rewrite - (Hcl ids). *)
-  (*     rewrite - (Hcl ids (to_subst ρ) ). *)
-  (*     asimpl. *)
-  (*     iApply "H". *)
-  (*   } *)
-
-  (*     (* ("Hclosed" $! (to_subst ρ) ids) as "#H2". *) *)
-  (*     (* iRewrite "#H2". *) *)
-
-  (*     (* iPoseProof ("Hclosed" $! (to_subst ρ) ids) as "#H2". *) *)
-  (*     (* iRewrite "#H2". *) *)
-  (*   iSplit; iIntros "/= #Htp !> * #Hg"; *)
-  (*     iSpecialize ("Htp" $! ρ); iSpecialize ("Hren" $! ρ with "Hg"). *)
-  (*   -  *)
-  (*     iApply "Hren". *)
-  (*     by iApply "Htp". *)
-  (*   - iApply "Hren". *)
-  (*     by iApply "Htp". *)
-  (* Qed. *)
+    iSplit; iIntros "/= #[% #Htp]"; iSplit => //; iIntros " !> * #Hg";
+    iApply interp_subst_closed => //; by iApply "Htp".
+  Qed.
 
   Lemma ivstp_rec_i T v:
     ((∀ ρ1 ρ2, (∀ x, x < length Γ → ρ1 x = ρ2 x) → v.[ρ1] = v.[ρ2]) ->
@@ -311,4 +289,5 @@ Section Sec.
     ivtp Γ (TMu T) v -∗
     ivtp Γ T.|[v/] v).
   Proof. by intros; iDestruct ivstp_rec_eq as "[? ?]". Qed.
+
 End Sec.
