theories/lr_lemmasTSel.v
@@ -18,11 +18,9 @@ Section Sec.
     ivtp Γ (TTMem l L U) va -∗
     Γ ⊨ L <: TSelA (pv va) l L U.
   Proof.
-    iIntros "#Hva".
-
-    iIntros "/= !> * Hg #HvL".
-    iDestruct ("Hva" $! ρ with "Hg") as (d) "#[% #H]"; iClear "Hva".
-    iDestruct "H" as (φ σ) "#[Hl [#HLφ [#HφU #HLU]]]".
+    iIntros "/= #[% #Hva] !> * #Hg #HvL".
+    iDestruct ("Hva" $! ρ with "Hg") as (Hclva d Hl Hcld φ σ) "#H"; iClear "Hva".
+    iDestruct "H" as "#[Hl [#HLφ [#HφU #HLU]]]".
     repeat iSplit; first by iApply "HLU".
     iRight.
     iExists σ, φ, d.
@@ -33,38 +31,37 @@ Section Sec.
 
   Lemma mem_stp_sel_sub L U va l:
     ivtp Γ (TTMem l L U) va -∗
-    ivstp Γ (TLater L) (TSel (pv va) l).
+    Γ ⊨ TLater L <: TSel (pv va) l.
   Proof.
-    iIntros "/= #Hva !> * #Hg #HvL".
-    iDestruct ("Hva" $! ρ with "Hg") as (d) "#[% #H]"; iClear "Hva".
-    iDestruct "H" as (φ σ) "#[Hl [#HLφ [#HφU #HLU]]]".
-    repeat iSplit; first done.
+    iIntros "/= #[% Hva] !> * #Hg #[% HvL]".
+    iDestruct ("Hva" $! ρ with "Hg") as (Hclva d Hl Hcld φ σ) "#H"; iClear "Hva".
+    iDestruct "H" as "#[Hl [#HLφ [#HφU #HLU]]]".
+    repeat iSplit => //.
     iRight.
     iExists σ , φ, d.
     iDestruct ("HLφ" with "HvL") as "#HLφ'".
     repeat iModIntro; by repeat iSplit.
   Qed.
 
-  Instance Inhϕ: Inhabited (list vl * vl → iProp Σ).
-  Proof. constructor. exact (λ _, False)%I. Qed.
+  Instance Inhϕ: Inhabited (listVlC -n> vlC -n> iProp Σ).
+  Proof. constructor. exact (λne _ _, False)%I. Qed.
 
   (* Next step: proper lemma on arbitrary-length paths. *)
   Lemma mem_stp_sel_sub_path1 L U va l1 l2:
     (ivtp Γ (TVMem l1 (TTMem l2 L U)) va -∗
     ivstp Γ (TLater L) ((TSel (pself (pv va) l1) l2)))%I.
   Proof.
-    iIntros "/= #Hva !> * #Hg #HvL".
+    iIntros "/= #[% Hva] !> * #Hg #[% HvL]".
 
-    iDestruct ("Hva" $! ρ with "Hg") as (d) "#[% #Hvb]"; iClear "Hva".
-    iDestruct "Hvb" as (vmem) "[-> H1]".
-    iDestruct "H1" as (d) "[Hl2 H]".
+    iDestruct ("Hva" $! ρ with "Hg") as (Hclva d Hl Hcld vmem) "#[-> #[_ H1]]"; iClear "Hva".
+    iDestruct "H1" as (d) "[Hl2 [_ H]]".
     iDestruct "H" as (φ σ) "#[Hl [#HLφ [#HφU #HLU]]]".
     iDestruct ("HLφ" with "HvL") as "HLφ'".
-    repeat iSplit; first done.
+    iSplit; first done.
     iRight.
     iExists vmem.
-    repeat iSplit; try done.
-    iExists σ , φ, d.
+    iSplit; try done.
+    iExists σ, φ, d.
     repeat iModIntro; by repeat iSplit.
   Qed.
 
@@ -72,14 +69,11 @@ Section Sec.
     ivtp Γ (TTMem l L U) va -∗
     ivstp Γ (TSel (pv va) l) (TLater U).
   Proof.
-    iIntros "/= #Hva !> * #Hg #[_ [[] | Hφ]]".
-    iDestruct ("Hva" $! ρ with "Hg") as (d) "#[% #H]"; iClear "Hva".
-    iDestruct "H" as (φ σ) "#[Hlφ [HLφ [HφU #HLU]]]".
-    iDestruct "Hlφ" as (γ) "[% Hγφ]".
-
+    iIntros "/= #[% Hva] !> * #Hg #[$ [[] | Hφ]]".
+    iDestruct ("Hva" $! ρ with "Hg") as (Hclva d Hl Hcld φ σ) "#[Hlφ [HLφ [HφU #HLU]]]"; iClear "Hva".
+    iDestruct "Hlφ" as (γ Hd) "Hγφ".
     iApply "HφU".
     iDestruct "Hφ" as (σ1 φ1 d1 Hva) "[Hγ #HΦ1v]".
-    (* " [_ [False | #HΦ1v]]]"; try done. *)
     iDestruct "Hγ" as (γ' Hd1) "HγΦ1".
 
     injectHyps; subst; objLookupDet.
